More progress with spawn.

concurrency/compiler/spawn_diagrams.v
@@ -104,9 +104,176 @@ Section SpawnDiagrams.
     Notation mtch_source:= (mtch_source hb).
 
 
+    Definition build_spwan_event addr dmap1 dmap2 m:=
+      Events.spawn addr (Some (build_delta_content dmap1 m))
+                   (Some (build_delta_content dmap2 m)).
+
+    
+    Lemma spawn_step_diagram_self Sem tid:
+      let CoreSem:= sem_coresem Sem in
+      forall (SelfSim: (self_simulation (@semC Sem) CoreSem))
+        virtue1 virtue_new1 (m1 m2 : mem) cd
+        (mu : meminj) (st1 : ThreadPool (Some hb)) 
+        (st2 : ThreadPool (Some (S hb)))
+        (cnt1 : ThreadPool.containsThread(Sem:=HybridSem _) st1 tid)
+        (cnt2 : containsThread(Sem:=HybridSem _) st2 tid)
+        (c : semC) (b1 b2 : block) (ofs : int) delt arg
+        (Hneq: tid <> hb )
+        (Hinj_b : mu b1 = Some (b2, delt))
+        (CMatch: concur_match cd mu st1 m1 st2 m2)
+        
+        (* Thread states *)
+        (th_state1: @semC Sem) th_state2 sum_state1 sum_state2
+        (HState1: coerce_state_type _ sum_state1 th_state1  
+                                    (CSem, Clight.state) (AsmSem,Asm.state) (Sem,@semC Sem))
+        (HState2: coerce_state_type _ sum_state2 th_state2
+                                    (CSem, Clight.state) (AsmSem,Asm.state) (Sem,@semC Sem))
+        (Hget_th_state1: @getThreadC _ _ tid st1 cnt1 = Kblocked sum_state1)
+        (Hget_th_state2: @getThreadC _ _ tid st2 cnt2 = Kblocked sum_state2)
+        (Amatch : match_self (code_inject _ _ SelfSim) mu th_state1 m1 th_state2 m2)
+
+        
+        (Hthread_mem1: access_map_equiv (thread_perms _ _ cnt1) (getCurPerm m1))
+        (Hthread_mem2: access_map_equiv (thread_perms _ _ cnt2) (getCurPerm m2))
+        
+        (Harg : val_inject (Mem.flat_inj (Mem.nextblock m1)) arg arg),
+        let ThreadPerm1:= (computeMap_pair (getThreadR cnt1) virtue1) in
+        let newThreadPerm1:= (computeMap_pair (pair0 empty_map) virtue_new1) in
+
+        let st1':= (ThreadPool.updThread cnt1 (Kresume c Vundef) ThreadPerm1) in
+        let st1'':= (ThreadPool.addThread st1' (Vptr b1 ofs) arg newThreadPerm1) in
+        forall (Hcmpt : mem_compatible  st1'' m1)
+          (Hinv' : invariant st1'')
+          (Hangel_bound: pair21_prop sub_map virtue1 (snd (getMaxPerm m1)))
+          (Hangel_bound_new : pair21_prop sub_map virtue_new1 (snd (getMaxPerm m1)))
+          (Amatch : match_self (code_inject _ _ SelfSim) mu th_state1 m1 th_state2 m2)
+          (Hmatch_mem: match_mem mu m1 m2)
+          (Hat_external: semantics.at_external CoreSem th_state1 m1 =
+                         Some (FREE_LOCK, (Vptr b1 ofs :: nil)%list))
+          (Hjoin_angel: permMapJoin_pair newThreadPerm1 ThreadPerm1 (getThreadR cnt1)),
+
+        exists evnt2 (st2'' : t) m2',
+          let evnt:= build_spwan_event (b1, unsigned ofs)
+                                       (fst virtue1)
+                                       (fst virtue_new1)
+                                       m1 in 
+          concur_match cd mu st1'' m1 st2'' m2' /\
+          inject_sync_event mu evnt evnt2 /\
+          let Hcmpt2:=  (memcompat2 CMatch) in
+          syncStep(Sem:=HybridSem (Some (S hb)))
+                  true cnt2 Hcmpt2 st2'' m2' evnt2.
+    Proof.
+    Admitted.
+
+    
+    Lemma spawn_step_diagram:
+      let hybrid_sem:= (sem_coresem (HybridSem (Some hb))) in 
+      forall virtue1 virtue_new1 (m1 m2 : mem) (tid : nat) cd
+        (mu : meminj) (st1 : ThreadPool (Some hb)) 
+        (st2 : ThreadPool (Some (S hb)))
+        (cnt1 : ThreadPool.containsThread(Sem:=HybridSem _) st1 tid)
+        (cnt2 : containsThread(Sem:=HybridSem _) st2 tid)
+        (c : semC) (b : block) (ofs : int) arg
+        (Hthread_mem1: access_map_equiv (thread_perms _ _ cnt1) (getCurPerm m1))
+        (Hthread_mem2: access_map_equiv (thread_perms _ _ cnt2) (getCurPerm m2))
+        (CMatch: concur_match cd mu st1 m1 st2 m2)
+        (Hcode: getThreadC cnt1 = Kblocked c)
+        (Harg : val_inject (Mem.flat_inj (Mem.nextblock m1)) arg arg),
+        let ThreadPerm1:= (computeMap_pair (getThreadR cnt1) virtue1) in
+        let newThreadPerm1:= (computeMap_pair (pair0 empty_map) virtue_new1) in
+
+        let st1':= (ThreadPool.updThread cnt1 (Kresume c Vundef) ThreadPerm1) in
+        let st1'':= (ThreadPool.addThread st1' (Vptr b ofs) arg newThreadPerm1) in
+        forall (Hcmpt : mem_compatible  st1'' m1)
+          (Hinv' : invariant st1'')
+          (Hangel_bound: pair21_prop sub_map virtue1 (snd (getMaxPerm m1)))
+          (Hangel_bound_new : pair21_prop sub_map virtue_new1 (snd (getMaxPerm m1)))
+          (Hat_external: semantics.at_external hybrid_sem c m1 =
+                         Some (CREATE, Vptr b ofs :: arg :: nil))
+          (Hjoin_angel: permMapJoin_pair newThreadPerm1 ThreadPerm1 (getThreadR cnt1)),
+
+        exists evnt2 (st2'' : t) m2',
+          let evnt:= build_spwan_event (b, unsigned ofs)
+                                       (fst virtue1)
+                                       (fst virtue_new1)
+                                       m1 in 
+          concur_match cd mu st1'' m1 st2'' m2' /\
+          inject_sync_event mu evnt evnt2 /\
+          let Hcmpt2:=  (memcompat2 CMatch) in
+          syncStep(Sem:=HybridSem (Some (S hb)))
+                  true cnt2 Hcmpt2 st2'' m2' evnt2.
+    Proof.
+      intros; simpl in *.
+      get_mem_compatible.
+      get_thread_mems.
+      clean_proofs.
+
+      pose proof (cur_equiv_restr_mem_equiv
+                    _ _ (th_comp thread_compat1) Hthread_mem1) as
+          Hmem_equiv.
+      
+      (* destruct {tid < hb} + {tid = hb} + {hb < tid}  *)
+      destruct (Compare_dec.lt_eq_lt_dec tid hb) as [[?|?]|?].
+
+      - (* (tid < hb) *)
+        pose proof (mtch_target _ _ _ _ _ _ CMatch _ l cnt1 (contains12 CMatch cnt1))
+          as match_thread.
+        simpl in Hcode; exploit_match ltac:(apply CMatch).
+        inversion H3. (* Asm_match *)
+        
+        (*Destruct the values of the self simulation *)
+        pose proof (self_simulation.minject _ _ _ matchmem) as Hinj.
+        assert (Hinj':=Hinj).
+        pose proof (self_simulation.ssim_external _ _ Aself_simulation) as sim_atx.
+        eapply sim_atx in Hinj'; eauto.
+        2: { (*at_external*)
+          simpl. replace (restrPermMap Hlt1) with m1.
+          2:{  rewrite self_restre_eq; eauto. }
+          move Hat_external at bottom.
+          eauto.
+          
+               rewrite Hthread_mem1.
+            
+          erewrite restr_proof_irr.
+          rewrite Hmem_equiv; simpl; eassumption.
+        }
+        clear sim_atx.
+        destruct Hinj' as (b' & delt & Hinj_b & Hat_external2); eauto.
+        (* bounded_nat_func' pdata LKSIZE_nat *)
+        (edestruct (free_step_diagram_self AsmSem tid) as
+            (e' & Hthread_match & CMatch' & Htrace_inj & external_step)); eauto;
+          first[ eassumption|
+                 econstructor; eassumption|
+                 solve[econstructor; eauto] |
+                 eauto].
+        + omega.
+        + !goal (access_map_equiv _ _). clean_proofs; eassumption.
+        + (*match_self*)
+          econstructor.
+          * eapply cinject.
+          * simpl. move matchmem at bottom.
+            eapply match_mem_proper; try eapply matchmem; eauto.
+            -- symmetry; eapply cur_equiv_restr_mem_equiv; eauto.
+            -- symmetry; eapply cur_equiv_restr_mem_equiv; eauto.
+               clean_proofs; eauto.
+        + exists e'; eexists; exists m2.
+          repeat weak_split eauto.
+          (* * (* reestablish concur *)
+            rename b into BB.
+            !goal (concur_match _ _ (remLockfFullUpdate _ _ _ _ _ _ ) _ _ _).
+            simpl; eauto.
+          * clear - Htrace_inj; auto.*)
+          * clean_proofs; eauto.
+            
+            
+            
+
+            
+            
+    Admitted.
 
     (** * Here be dragons  *)
 
     
-    End spawn.
+  End spawn.
 End SpawnDiagrams.
